Implement Shareable type class and instances, #37 and #38

Coq/src/DataM.v
@@ -1,58 +1,5 @@
+Require Import Thesis.Container.
 Require Import Thesis.Free.
-Require Import Thesis.Effect.
 Require Import Thesis.Base.
 
 Set Implicit Arguments.
-
-Section Pair.
-  Inductive Pair A B :=
-  | Pair' : Prog A -> Prog B -> Pair A B.
-  
-  Definition pairM A B (fst : Prog A) (snd : Prog B) : Prog (Pair A B) :=
-    pure (Pair' fst snd).
-
-  Definition first A B (fp : Prog (Pair A B)) : Prog A :=
-    fp >>= fun '(Pair' fst _) => fst.
-
-  Definition second A B (fp : Prog (Pair A B)) : Prog B :=
-    fp >>= fun '(Pair' _ snd) => snd.
-
-  Definition dup' (fp : Prog (Pair bool bool)) : Prog (Pair bool bool) :=
-    pairM (first fp) (first fp).
-
-  Definition dup A (fx : Prog A) : Prog (Pair A A) :=
-    pairM fx fx.
-
-  Definition dupShare A (fx : Prog A) : Prog (Pair A A) :=
-    Share fx >>= fun x => pairM x x.
-End Pair.
-
-Section List.
-  Inductive List A :=
-  | Nil : List A
-  | Cons : Prog A -> Prog (List A) -> List A.
-
-  Definition cons A (fx : Prog A) (fxs : Prog (List A)) : Prog (List A) :=
-    pure (Cons fx fxs).
-
-  Definition nil A : Prog (List A) := pure (@Nil A).
-
-  Definition headM A (fxs : Prog (List A)) : Prog A :=
-    fxs >>= fun xs => match xs with
-                   | Nil _    => Fail
-                   | Cons x _ => x
-                   end.
-
-  Definition dupl A (fx : Prog A) : Prog (List A) :=
-    cons fx (cons fx (@nil A)).
-
-  Definition duplShare A (fx : Prog A) : Prog (List A) :=
-    Share fx >>= fun x => cons x (cons x (@nil A)).
-
-  (* Fixpoint appM A (fxs fys : Prog (List A)) : Prog (List A) := *)
-  (*   fxs >>= fun xs => match xs with *)
-  (*                  | Nil _       => fys *)
-  (*                  | Cons fz fzs => cons fz (appM fzs fys) *)
-  (*                  end. *)
-
-End List.
