Coq/src/Effect.v
@@ -1,34 +1,23 @@
+Require Import Thesis.Base.
 Require Import Thesis.Container.
 Require Import Thesis.Free.
-Require Import Thesis.Base.
 
 Set Implicit Arguments.
 
-Definition NDShare := C__Comb (C__State nat) (C__Comb C__Sharing C__Choice).
-
-Definition NDShare__SC := C__Comb C__Sharing C__Choice.
-
-Definition Prog := Free NDShare.
-
-Definition Prog__SC := Free NDShare__SC.
-
-Definition Fail A : Prog A :=
-  let s : @Shape _ NDShare := inr (inr sfail)
-  in impure (ext s (fun p : @Pos _ NDShare s => match p with end)).
-
-Arguments Fail {_}.
-
-Definition Fail__C A : Free C__Choice A :=
-  let s : @Shape _ C__Choice := sfail
-  in impure (ext s (fun p : Pos__Choice s => match p with end)).
-
-Arguments Fail__C {_}.
-
-Definition Fail__SC A : Free (C__Comb C__Sharing C__Choice) A :=
-  let s : @Shape _ NDShare__SC := inr sfail
-  in impure (ext s (fun p : @Pos _ NDShare__SC s => match p with end)).
-
-Arguments Fail__SC {_}.
+Section Prog.
+  Definition NDShare := C__Comb (C__State nat) (C__Comb C__Sharing C__Choice).
+  
+  Definition NDShare__SC := C__Comb C__Sharing C__Choice.
+  
+  Definition Prog := Free NDShare.
+  
+  Definition Prog__SC := Free NDShare__SC.
+End Prog.
+ 
+Class Shareable (A : Type) :=
+  {
+    shareArgs : A -> Prog A
+  }.
 
 Definition Get : Prog nat :=
   let s : @Shape _ NDShare := inl (sget nat)
@@ -46,8 +35,27 @@ Definition Share'__SC (n : nat) A (fs : Prog__SC A) : Prog__SC A :=
   let s : @Shape _ NDShare__SC := inl (ssharing n)
   in impure (ext s (fun p : @Pos _ NDShare__SC s => fs)).
 
-Definition Share A (fp : Prog A) : Prog (Prog A) :=
-  Get >>= fun i => Put (i * 2) >>= fun _=> pure (Share' i (Put (i * 2 + 1) >>= fun _ => fp)).
+Definition Share A `(Shareable A) (fp : Prog A) : Prog (Prog A) :=
+  Get >>= fun i => Put (i * 2) >>= fun _=> pure (Share' i (Put (i * 2 + 1) >>= fun _ => fp >>= fun x => shareArgs x)).
+Arguments Share {_} {_} fp.
+
+Definition Fail A : Prog A :=
+  let s : @Shape _ NDShare := inr (inr sfail)
+    in impure (ext s (fun p : @Pos _ NDShare s => match p with end)).
+
+Arguments Fail {_}.
+
+Definition Fail__C A : Free C__Choice A :=
+  let s : @Shape _ C__Choice := sfail
+  in impure (ext s (fun p : Pos__Choice s => match p with end)).
+
+Arguments Fail__C {_}.
+
+Definition Fail__SC A : Free (C__Comb C__Sharing C__Choice) A :=
+  let s : @Shape _ NDShare__SC := inr sfail
+  in impure (ext s (fun p : @Pos _ NDShare__SC s => match p with end)).
+
+Arguments Fail__SC {_}.
 
 Definition Choice__C A mid l r : Free C__Choice A :=
   let s : @Shape _ C__Choice := schoice mid
@@ -60,3 +68,106 @@ Definition Choice__SC A mid l r : Prog__SC A :=
 Definition Choice A mid l r : Prog A :=
   let s : @Shape _ NDShare := inr (inr (schoice mid))
   in impure (ext s (fun p : @Pos _ NDShare s => if p then l else r)).
+
+Section Pair.
+  Inductive Pair A B :=
+  | Pair' : Prog A -> Prog B -> Pair A B.
+  
+  Definition pairM A B (fst : Prog A) (snd : Prog B) : Prog (Pair A B) :=
+    pure (Pair' fst snd).
+
+  Definition first A B (fp : Prog (Pair A B)) : Prog A :=
+    fp >>= fun '(Pair' fst _) => fst.
+
+  Definition second A B (fp : Prog (Pair A B)) : Prog B :=
+    fp >>= fun '(Pair' _ snd) => snd.
+
+  Definition dup' (fp : Prog (Pair bool bool)) : Prog (Pair bool bool) :=
+    pairM (first fp) (first fp).
+
+  Definition dup A (fx : Prog A) : Prog (Pair A A) :=
+    pairM fx fx.
+
+  Definition dupShare A `(Shareable A) (fx : Prog A) : Prog (Pair A A) :=
+    Share fx >>= fun x => pairM x x.
+
+  Definition shrrgs__Pair A B `(Shareable A) `(Shareable B) (p : Pair A B) : Prog (Pair A B) :=
+    match p with
+    | Pair' a b => Share a >>= fun sa => Share b >>= fun sb => pairM sa sb
+    end.
+
+  Global Instance shrbl__Pair A B `(sa : Shareable A) `(sb : Shareable B) : Shareable (Pair A B) :=
+    {
+      shareArgs := @shrrgs__Pair A B sa sb
+    }.
+End Pair.
+
+Section List.
+  Inductive List A :=
+  | Nil : List A
+  | Cons : Prog A -> Prog (List A) -> List A.
+
+  Definition cons A (fx : Prog A) (fxs : Prog (List A)) : Prog (List A) :=
+    pure (Cons fx fxs).
+
+  Definition nil A : Prog (List A) := pure (@Nil A).
+
+  Definition headM A (fxs : Prog (List A)) : Prog A :=
+    fxs >>= fun xs => match xs with
+                   | Nil _    => @Fail A
+                   | Cons x _ => x
+                   end.
+
+  Definition dupl A (fx : Prog A) : Prog (List A) :=
+    cons fx (cons fx (@nil A)).
+
+  Definition duplShare A `(Shareable A) (fx : Prog A) : Prog (List A) :=
+    Share fx >>= fun x => cons x (cons x (@nil A)).
+
+  Fixpoint appM' A (xs : List A) (fxs : Prog (List A)) : Prog (List A) :=
+    match xs with
+    | Nil _       => fxs
+    | Cons fz fzs => cons fz (fzs >>= fun zs => appM' zs fxs)
+    end.
+
+  Fixpoint appM A (fxs fys : Prog (List A)) : Prog (List A) :=
+    fxs >>= fun xs => appM' xs fys.
+
+  Definition shrrgs__List A `(Shareable A) `(Shareable (List A)) (xs : List A) : Prog (List A) :=
+    match xs with
+    | Nil _     => @nil A
+    | Cons y ys => Share y >>= fun sy => Share ys >>= fun sys => cons sy sys
+    end.
+  
+  Global Instance shrbl__List A `(sa : Shareable A) (sas : Shareable (List A)) : Shareable (List A) :=
+    {
+      shareArgs := @shrrgs__List A sa sas
+    }.
+End List.
+
+Section Prim.
+  Definition Coin : Prog nat := Choice None (pure 0) (pure 1).
+  Definition Coin__Bool : Prog bool := Choice None (pure true) (pure false).
+  
+  Definition addM (fn1 fn2 : Prog nat) : Prog nat :=
+    fn1 >>= fun n1 => fn2 >>= fun n2 => pure (n1 + n2).
+  
+  Definition orM (fn1 fn2 : Prog bool) : Prog bool :=
+    fn1 >>= fun b => match b with
+                  | true => pure true
+                  | false => fn2
+                  end.
+  
+  Definition duplicate A (fx : Prog A) : Prog (A * A) :=
+    fx >>= fun x => fx >>= fun y => pure (x,y).
+End Prim.
+
+Global Instance shrbl__Nat : Shareable nat :=
+  {
+    shareArgs := pure
+  }.
+
+Global Instance shrbl__Bool : Shareable bool :=
+  {
+    shareArgs := pure
+  }.
