Coq/src/Handler.v
@@ -51,28 +51,3 @@ Fixpoint runSharing A (fs : Free (C__Comb C__Sharing C__Choice) A) : Free C__Cho
 
 Definition handle A (fs : Free NDShare A) : list A :=
   collectVals (runChoice (runSharing (runState 1 fs))).
-
-Section Examples.
-  Definition Coin : Free NDShare nat := Choice None (pure 0) (pure 1).
-  Definition Coin__Bool : Free NDShare bool := Choice None (pure true) (pure false).
-
-  Definition addM (fn1 fn2 : Free NDShare nat) : Free NDShare nat :=
-    fn1 >>= fun n1 => fn2 >>= fun n2 => pure (n1 + n2).
-
-  Definition orM (fn1 fn2 : Free NDShare bool) : Free NDShare bool :=
-    fn1 >>= fun b => match b with
-                  | true => pure true
-                  | false => fn2
-                  end.
-
-  Definition duplicate A (fx : Free NDShare A) : Free NDShare (A * A) :=
-    fx >>= fun x => fx >>= fun y => pure (x,y).
-
-  Example e1 : Free NDShare (nat * nat) := Share Coin >>= fun x => duplicate x.
-  
-  Example e2 : Free NDShare nat := Share Coin >>= fun x => addM x x.
-
-  Example e3 : Free NDShare bool := orM (pure true) Fail.
-  Eval compute in handle e3.
-
-End Examples.
