Coq/src/Example.v
@@ -1,0 +1,17 @@
+Require Import Thesis.Handler.
+Require Import Thesis.Effect.
+Require Import Thesis.Free.
+Require Import Thesis.Base.
+
+Set Implicit Arguments.
+
+Example p1 : Prog (nat * nat) := Share Coin >>= fun x => duplicate x.
+Lemma l1 : handle e1 = ((0, 0) :: (1, 1) :: Datatypes.nil)%list.
+
+Example e2 : Prog nat := Share Coin >>= fun x => addM x x.
+Lemma l2 : handle e2 = (0 :: 2 :: Datatypes.nil)%list.
+
+Example e3 : Prog bool := orM (pure true) Fail.
+Lemma l3 : handle e3 = (true :: Datatypes.nil)%list.
+
+Definition ls := (l1 :: l2 :: l3 :: Datatypes.nil)%list.
